Seccompjit.v
@@ -16,46 +16,41 @@ Definition id_mem: ident := 3%positive.
 
 Definition u32: type := Tint I32 Unsigned noattr.
 
-Fixpoint transf_code (src: Seccomp.code) (n: label) : res statement :=
+Open Local Scope error_monad_scope.
+
+Fixpoint transl_code (src: Seccomp.code) (n: label) : res statement :=
   match src with
   | nil => OK Sskip
-  | hd::tl => match transf_code tl (Psucc n) with
-    | Error msg => Error msg
-    | OK bodytl =>
-      match (match hd with
-      | Salu_add_k k =>
-        OK (Sset id_a (Ebinop Oadd (Etempvar id_a u32) (Econst_int k u32) u32))
-      | Sret_k k =>
-        OK (Sreturn (Some (Econst_int k u32)))
-      | Sret_a =>
-        OK (Sreturn (Some (Etempvar id_a u32)))
-      | _ => Error (msg "FIXME")
-      end) with
+  | hd::tl =>
+    do bodytl <- transl_code tl (Psucc n);
+    match (match hd with
+    | Salu_add_k k =>
+      OK (Sset id_a (Ebinop Oadd (Etempvar id_a u32) (Econst_int k u32) u32))
+    | Sret_k k =>
+      OK (Sreturn (Some (Econst_int k u32)))
+    | Sret_a =>
+      OK (Sreturn (Some (Etempvar id_a u32)))
+    | _ => Error (msg "FIXME")
+    end) with
       | Error msg => Error msg
       | OK bodyhd => OK (Slabel n (Ssequence bodyhd bodytl))
-      end
     end
   end.
 
-Definition transf_function (f: Seccomp.function) : res Clight.function :=
-  match transf_code f xH with
-  | Error msg => Error msg
-  | OK body =>
-    let vars := (id_mem, Tarray u32 seccomp_memwords noattr)::nil in
-    let temps := (id_a, u32)::(id_x, u32)::nil in
-    (* FIXME: memset(mem, 0, sizeof(mem)) *)
-    let body := Ssequence (Sset id_x (Econst_int Int.zero u32)) body in
-    let body := Ssequence (Sset id_a (Econst_int Int.zero u32)) body in
-    OK (Clight.mkfunction u32 nil vars temps body)
-  end.
+Definition transl_function (f: Seccomp.function) : res Clight.function :=
+  do body <- transl_code f xH;
+  let vars := (id_mem, Tarray u32 seccomp_memwords noattr)::nil in
+  let temps := (id_a, u32)::(id_x, u32)::nil in
+  (* FIXME: memset(mem, 0, sizeof(mem)) *)
+  let body := Ssequence (Sset id_x (Econst_int Int.zero u32)) body in
+  let body := Ssequence (Sset id_a (Econst_int Int.zero u32)) body in
+  OK (Clight.mkfunction u32 nil vars temps body).
 
-Open Local Scope error_monad_scope.
-
-Definition transf_fundef (fd: Seccomp.fundef) : res Clight.fundef :=
+Definition transl_fundef (fd: Seccomp.fundef) : res Clight.fundef :=
   match fd with
-  | AST.Internal f => do f' <- transf_function f; OK (Clight.Internal f')
+  | AST.Internal f => do f' <- transl_function f; OK (Clight.Internal f')
   | _ => Error (msg "external function not allowed")
   end.
 
-Definition transf_program (p: Seccomp.program) : res Clight.program :=
-  transform_partial_program transf_fundef p.
+Definition transl_program (p: Seccomp.program) : res Clight.program :=
+  transform_partial_program transl_fundef p.
