Seccompproof.v
@@ -1,47 +1,70 @@
 Require Import compcert.cfrontend.Clight.
+Require Import compcert.cfrontend.Ctypes.
 Require Import compcert.common.AST.
 Require Import compcert.common.Errors.
 Require Import compcert.common.Globalenvs.
+Require Import compcert.common.Memory.
 Require Import compcert.common.Values.
+Require Import compcert.lib.Coqlib.
 Require Import Seccomp.
 Require Import Seccompjit.
 
-Section PRESERVATION.
+(* Section PRESERVATION. *)
 
 Variable prog: Seccomp.program.
 Variable tprog: Clight.program.
-Hypothesis TRANSF: transf_program prog = OK tprog.
+Hypothesis TRANSL: transl_program prog = OK tprog.
 Let ge := Genv.globalenv prog.
 Let tge := Genv.globalenv tprog.
 
 Lemma symbols_preserved:
   forall (s: ident), Genv.find_symbol tge s = Genv.find_symbol ge s.
 Proof.
-  exact (Genv.find_symbol_transf_partial _ _ TRANSF).
+  exact (Genv.find_symbol_transf_partial _ _ TRANSL).
+Qed.
+
+Lemma function_ptr_translated:
+  forall (b: block) (f: fundef),
+  Genv.find_funct_ptr ge b = Some f ->
+  exists tf, Genv.find_funct_ptr tge b = Some tf /\ transl_fundef f = OK tf.
+Proof.
+  exact (Genv.find_funct_ptr_transf_partial _ _ TRANSL).
+Qed.
+
+Lemma sig_translated:
+  forall fd tfd,
+  transl_fundef fd = OK tfd ->
+  Clight.type_of_fundef tfd = Tfunction Tnil u32.
+Proof.
+  intros.
+  destruct fd; monadInv H.
+  destruct f; monadInv EQ; auto.
 Qed.
 
 Inductive match_states: Seccomp.state -> Clight.state -> Prop :=
   | match_state:
-      forall a x m f pc tf s k e le tm,
-      match_states (Seccomp.State a x m f pc)
+      forall a x sm f pc m tf s k e le tm,
+      match_states (Seccomp.State a x sm f pc m)
                    (Clight.State tf s k e le tm)
   | match_callstate:
-      forall f tf args k tm
-        (TF: transf_fundef f = OK tf)
-        ,
-      match_states (Seccomp.Callstate f)
-                   (Clight.Callstate tf args k tm)
+      forall fd m tfd args k tm
+        (TF: transl_fundef fd = OK tfd)
+        (MCONT: k = Kstop)
+        (MARGS: args = nil)
+        (MEXT: Mem.extends m tm),
+      match_states (Seccomp.Callstate fd m)
+                   (Clight.Callstate tfd args k tm)
   | match_returnstate:
-      forall v tv k tm
+      forall v m tv k tm
         (MV: Vint v = tv),
-      match_states (Seccomp.Returnstate v)
+      match_states (Seccomp.Returnstate v m)
                    (Clight.Returnstate tv k tm)
   .
 
 (*
-Lemma transf_initial_states:
+Lemma transl_initial_states:
   forall S, Seccomp.initial_state prog S ->
   exists R, Clight.initial_state tprog R /\ match_states S R.
 *)
 
-End PRESERVATION.
+(* End PRESERVATION. *)
